Work on SSA formalization

FreydSSA/Basic.lean
@@ -1,4 +1,10 @@
 import Mathlib.Data.List.Basic
+import Std.Data.List.Basic
+import Mathlib.Data.Set.Basic
+import Mathlib.Data.Set.Function
+import Mathlib.Init.Classical
+
+open List.«term_<+_»
 
 structure Var (ν : Type u) (α : Type v) : Type (max u v) where
   name: ν
@@ -6,31 +12,39 @@ structure Var (ν : Type u) (α : Type v) : Type (max u v) where
 
 def Ctx (ν: Type u) (α: Type v): Type (max u v) := List (Var ν α)
 
-inductive Ctx.notin {ν α} (n : ν) : Ctx ν α → Prop
-  | nil : Ctx.notin n []
-  | cons {Γ x} : x.name ≠ n → Ctx.notin n Γ → Ctx.notin n (x::Γ)
+@[simp]
+def Ctx.names {ν α} (Γ: Ctx ν α): List ν
+  := Γ.map Var.name
 
-theorem Ctx.notin.head {ν α} {n} {y : Var ν α} {Γ : Ctx ν α}
-  : Ctx.notin n (y::Γ) → y.name ≠ n
+inductive Ctx.Fresh {ν α} (n : ν) : Ctx ν α → Prop
+  | nil : Ctx.Fresh n []
+  | cons {Γ x} : x.name ≠ n → Ctx.Fresh n Γ → Ctx.Fresh n (x::Γ)
+
+theorem Ctx.Fresh.head {ν α} {n} {y : Var ν α} {Γ : Ctx ν α}
+  : Ctx.Fresh n (y::Γ) → y.name ≠ n
   | cons hxn _ => hxn
 
-inductive Ctx.wk {ν: Type u} {α: Type v} : Ctx ν α → Ctx ν α → Type (max u v)
-  | nil : Ctx.wk [] []
-  | cons {Γ Δ} (x : Var ν α) : Ctx.wk Γ Δ → Ctx.wk (x::Γ) (x::Δ)
-  | skip {Γ Δ} : Ctx.notin x.name Δ → Ctx.wk Γ Δ → Ctx.wk (x::Γ) Δ
+theorem Ctx.Fresh.tail {ν α} {n} {y : Var ν α} {Γ : Ctx ν α}
+  : Ctx.Fresh n (y::Γ) → Ctx.Fresh n Γ
+  | cons _ hn => hn
 
-theorem Ctx.notin.wk {ν α} {Γ Δ: Ctx ν α} {n: ν}: notin n Γ → Γ.wk Δ → notin n Δ
-  | _, wk.nil => nil
-  | cons hxn hn, wk.cons _ h => cons hxn (hn.wk h)
-  | cons _ hn, wk.skip _ h => hn.wk h
+inductive Ctx.Wk {ν: Type u} {α: Type v} : Ctx ν α → Ctx ν α → Type (max u v)
+  | nil : Ctx.Wk [] []
+  | cons {Γ Δ} (x : Var ν α) : Ctx.Wk Γ Δ → Ctx.Wk (x::Γ) (x::Δ)
+  | skip {Γ Δ} : Ctx.Fresh x.name Δ → Ctx.Wk Γ Δ → Ctx.Wk (x::Γ) Δ
 
-def Ctx.wk.comp {ν α} {Γ Δ Ξ : Ctx ν α} : Γ.wk Δ → Δ.wk Ξ → Γ.wk Ξ
+theorem Ctx.Fresh.wk {ν α} {Γ Δ: Ctx ν α} {n: ν}: Fresh n Γ → Γ.Wk Δ → Fresh n Δ
+  | _, Wk.nil => nil
+  | cons hxn hn, Wk.cons _ h => cons hxn (hn.wk h)
+  | cons _ hn, Wk.skip _ h => hn.wk h
+
+def Ctx.Wk.comp {ν α} {Γ Δ Ξ : Ctx ν α} : Γ.Wk Δ → Δ.Wk Ξ → Γ.Wk Ξ
   | nil, h => h
   | cons x h, cons _ h' => cons x (h.comp h')
   | cons _ h, skip hn h' => skip hn (h.comp h')
   | skip hn h, h' => skip (hn.wk h') (h.comp h')
 
-theorem Ctx.wk.allEq {ν α} {Γ Δ : Ctx ν α} (D D': Γ.wk Δ): D = D'
+theorem Ctx.Wk.allEq {ν α} {Γ Δ : Ctx ν α} (D D': Γ.Wk Δ): D = D'
   := by induction D with
   | nil => cases D'; rfl
   | cons _ _ I => cases D' with
@@ -40,7 +54,7 @@ theorem Ctx.wk.allEq {ν α} {Γ Δ : Ctx ν α} (D D': Γ.wk Δ): D = D'
     | cons _ _ => exact (hxn.head rfl).elim
     | skip h I' => exact congrArg _ (I I')
 
-def Ctx.wk.refl {ν α}: (Γ : Ctx ν α) → Γ.wk Γ
+def Ctx.Wk.refl {ν α}: (Γ : Ctx ν α) → Γ.Wk Γ
   | [] => nil
   | x::Γ => cons x (refl Γ)
 
@@ -62,62 +76,284 @@ instance : OfNat Purity 1 where
   ofNat := Purity.pure
 
 --TODO: make into struct parameter?
-class InstSet (α : Type u) : Type _ where
-  inst : Purity → α → α → Type
-  pure_to_impure : inst 1 a b -> inst 0 a b
+structure InstSet (α : Type u) : Type _ where
+  Op : Purity → α → α → Type
+  pure_to_impure : Op 1 a b → Op 0 a b
 
-def InstSet.to_impure {α : Type u} [InstSet α] {p} {a b : α} (f: inst p a b)
-  : inst 0 a b
+def InstSet.to_impure {α : Type u} (Φ : InstSet α) {p} {A B : α} (f : Φ.Op p A B)
+  : Φ.Op 0 A B
   := match p with
-  | Purity.pure => pure_to_impure f
+  | Purity.pure => Φ.pure_to_impure f
   | Purity.impure => f
 
-inductive Tm {ν : Type u} {α : Type v} [InstSet (Ty α)]
-  : Purity -> Ctx ν (Ty α) → Ty α → Type (max u v) where
-  | var (p) : Γ.wk [x] → Tm p Γ x.ty
-  | op (f: InstSet.inst p a b) : Tm 1 Γ a → Tm p Γ b
-  | pair (p) : Tm 1 Γ a → Tm 1 Γ b → Tm p Γ (Ty.pair a b)
-  | unit (p) : Tm p Γ Ty.unit
+inductive InstSet.Tm {ν : Type u} {α : Type v} (Φ : InstSet (Ty α))
+  : Purity → Ctx ν (Ty α) → Ty α → Type (max u v) where
+  | var {x} (p) : Γ.Wk [x] → Tm Φ p Γ x.ty
+  | op (f: Φ.Op p A B) : Tm Φ 1 Γ A → Tm Φ p Γ B
+  | pair (p) : Tm Φ 1 Γ A → Tm Φ 1 Γ B → Tm Φ p Γ (Ty.pair A B)
+  | unit (p) : Tm Φ p Γ Ty.unit
 
-def Tm.to_impure [InstSet (Ty α)] {a: Ty α} : Tm p Γ a → Tm 0 Γ a
+def InstSet.Tm.to_impure (Φ : InstSet (Ty α)) {A : Ty α} : Φ.Tm p Γ A → Φ.Tm 0 Γ A
   | var p h => var 0 h
-  | op f e => op (InstSet.to_impure f) e
+  | op f e => op (Φ.to_impure f) e
   | pair p x y => pair 0 x y
   | unit p => unit 0
 
-def Tm.wk [InstSet (Ty α)] {a: Ty α} : Γ.wk Δ -> Tm p Δ a -> Tm p Γ a
+def InstSet.Tm.wk {Φ : InstSet (Ty α)} {A : Ty α} : Γ.Wk Δ → Φ.Tm p Δ A → Φ.Tm p Γ A
   | h, var p h' => var p (h.comp h')
   | h, op f e => op f (wk h e)
   | h, pair p x y => pair p (wk h x) (wk h y)
   | h, unit p => unit p
 
-inductive Body {ν: Type u} {α: Type v} [InstSet (Ty α)]
-  : Purity -> Ctx ν (Ty α) -> Ctx ν (Ty α) -> Type (max u v) where
-  | nil (p) : Γ.wk Δ -> Body p Γ Δ
-  | let1 : Tm p Γ a -> Body p (⟨x, a⟩::Γ) Δ -> Body p Γ Δ
-  | let2 : Tm p Γ (Ty.pair a b)
-    -> Body p (⟨x, b⟩::⟨y, a⟩::Γ) Δ
-    -> Body p Γ Δ
+inductive InstSet.Body {ν : Type u} {α : Type v} (Φ : InstSet (Ty α))
+  : Purity → Ctx ν (Ty α) → Ctx ν (Ty α) → Type (max u v) where
+  | nil (p) : Γ.Wk Δ → Body Φ p Γ Δ
+  | let1 : Φ.Tm p Γ a → Body Φ p (⟨x, a⟩::Γ) Δ → Body Φ p Γ Δ
+  | let2 : Φ.Tm p Γ (Ty.pair A B)
+    → Body Φ p (⟨x, A⟩::⟨y, B⟩::Γ) Δ
+    → Body Φ p Γ Δ
 
-def Body.to_impure {Γ Δ: Ctx ν (Ty α)} [InstSet (Ty α)] : Body p Γ Δ → Body 0 Γ Δ
+def InstSet.Body.to_impure {Φ : InstSet (Ty α)} {Γ Δ : Ctx ν (Ty α)}
+  : Φ.Body p Γ Δ → Φ.Body 0 Γ Δ
   | nil _ h => nil 0 h
   | let1 e b => let1 e.to_impure b.to_impure
   | let2 e b => let2 e.to_impure b.to_impure
 
-def Body.wk_entry {Γ Δ Ξ: Ctx ν (Ty α)} [InstSet (Ty α)]
-  : Γ.wk Δ -> Body p Δ Ξ -> Body p Γ Ξ
+def InstSet.Body.wk_entry {Φ : InstSet (Ty α)} {Γ Δ Ξ : Ctx ν (Ty α)}
+  : Γ.Wk Δ → Φ.Body p Δ Ξ → Φ.Body p Γ Ξ
   | h, nil p h' => nil p (h.comp h')
   | h, let1 e b => let1 (Tm.wk h e) (wk_entry (h.cons _) b)
   | h, let2 e b => let2 (Tm.wk h e) (wk_entry ((h.cons _).cons _) b)
 
-def Body.wk_exit {Γ Δ Ξ: Ctx ν (Ty α)} [InstSet (Ty α)]
-  : Body p Γ Δ -> Δ.wk Ξ -> Body p Γ Ξ
+def InstSet.Body.wk_exit {Φ : InstSet (Ty α)} {Γ Δ Ξ : Ctx ν (Ty α)}
+  : Φ.Body p Γ Δ → Δ.Wk Ξ → Φ.Body p Γ Ξ
   | nil p h, h' => nil p (h.comp h')
   | let1 e b, h' => let1 e (wk_exit b h')
   | let2 e b, h' => let2 e (wk_exit b h')
 
-def Body.cat {Γ Δ Ξ: Ctx ν (Ty α)} [InstSet (Ty α)]
-  : Body p Γ Δ -> Body p Δ Ξ -> Body p Γ Ξ
+def InstSet.Body.cat {Φ : InstSet (Ty α)} {Γ Δ Ξ : Ctx ν (Ty α)}
+  : Φ.Body p Γ Δ → Φ.Body p Δ Ξ → Φ.Body p Γ Ξ
   | nil p h, b => wk_entry h b
   | let1 e b, b' => let1 e (cat b b')
   | let2 e b, b' => let2 e (cat b b')
+
+def Ctx.Wk.names {ν α} {Γ Δ : Ctx ν α} : Γ.Wk Δ → Δ.names.Sublist Γ.names
+  | Wk.nil => List.Sublist.slnil
+  | Wk.cons _ h => h.names.cons₂ _
+  | Wk.skip _ h => h.names.cons _
+
+def Var.rename {ν ν' α} (ρ : ν → ν') (v : Var ν α) : Var ν' α
+  := ⟨ρ v.name, v.ty⟩
+
+theorem Var.rename_eq {ν ν' α} (v: Var ν α) (ρ₁ ρ₂: ν → ν')
+  : ρ₁ v.name = ρ₂ v.name → Var.rename ρ₁ v = Var.rename ρ₂ v
+  := by cases v; simp [rename]
+
+def Ctx.rename {ν ν' α} (ρ : ν → ν') (Γ : Ctx ν α) : Ctx ν' α
+  := Γ.map (Var.rename ρ)
+
+def Ctx.InjOn (ρ : ν → ν') (Γ : Ctx ν α) : Prop
+  := Set.InjOn ρ { x : ν | x ∈ Γ.names }
+
+theorem Ctx.injOn_empty (ρ : ν → ν') : Ctx.InjOn ρ (@List.nil (Var ν α))
+  := λ _ hx => match hx with .
+
+theorem Ctx.InjOn.tail {ρ: ν → ν'} {v} {Γ : Ctx ν α} (h: Ctx.InjOn ρ (v::Γ))
+  : Ctx.InjOn ρ Γ
+  := λ _ hx _ hy hxy => h (hx.tail _) (hy.tail _) hxy
+
+theorem Ctx.InjOn.head {ρ: ν → ν'} {v} {Γ : Ctx ν α} (h: Ctx.InjOn ρ (v::Γ))
+  : ∀x ∈ Γ.names, ρ x = ρ v.name → x = v.name
+  := λ _ hx hx' => h (hx.tail _) (by simp) hx'
+
+theorem Ctx.InjOn.head_ne {ρ : ν → ν'} {v} {Γ : Ctx ν α} (h : Ctx.InjOn ρ (v::Γ))
+  : ∀x ∈ Γ.names, x ≠ v.name → ρ x ≠ ρ v.name
+  := λ _ hx hx' => h.ne (hx.tail _) (by simp) hx'
+
+theorem Ctx.InjOn.cons {ρ : ν → ν'} {v : Var ν α} {Γ : Ctx ν α}
+  (hv : ∀x ∈ Γ.names, ρ x = ρ v.name → x = v.name) (h : Ctx.InjOn ρ Γ)
+  : Ctx.InjOn ρ (v::Γ)
+  | _, List.Mem.head _, _, List.Mem.head _, _ => rfl
+  | _, List.Mem.head _, _, List.Mem.tail _ ha, hav => (hv _ ha hav.symm).symm
+  | _, List.Mem.tail _ ha, _, List.Mem.head _, hav => hv _ ha hav
+  | _, List.Mem.tail _ hx, _, List.Mem.tail _ hy, hxy => h hx hy hxy
+
+theorem Ctx.InjOn.cons_ne {ρ : ν → ν'} {v : Var ν α} {Γ : Ctx ν α}
+  (hv : ∀x ∈ Γ.names, x ≠ v.name → ρ x ≠ ρ v.name) (h : Ctx.InjOn ρ Γ)
+  : Ctx.InjOn ρ (v::Γ)
+  := h.cons (λ_ hx hxv => Classical.by_contradiction (λh => hv _ hx h hxv))
+
+theorem Ctx.InjOn.wk {ρ : ν → ν'} {Γ : Ctx ν α} (hΓ : Γ.InjOn ρ) : Γ.Wk Δ → Δ.InjOn ρ
+  | Wk.nil => Ctx.injOn_empty _
+  | Wk.cons x h => (hΓ.tail.wk h).cons (λ_ hx hxv => hΓ.head _ (h.names.subset hx) hxv)
+  | Wk.skip _ h => hΓ.tail.wk h
+
+theorem Ctx.Fresh.rename {ν α} {ρ: ν → ν'} {Γ : Ctx ν α} {n}
+  (hΓ : Γ.InjOn ρ) (hn : ∀x ∈ Γ.names, x ≠ n → ρ x ≠ ρ n)
+  : Fresh n Γ → Fresh (ρ n) (rename ρ Γ)
+  | nil => nil
+  | cons hxn hn' => cons (hn _ (by simp) hxn) (hn'.rename hΓ.tail (λ x hx => hn _ (hx.tail _)))
+
+def Ctx.Wk.rename {ν α} {ρ : ν → ν'} {Γ Δ : Ctx ν α} (hΓ : Γ.InjOn ρ)
+  : Γ.Wk Δ → (rename ρ Γ).Wk (rename ρ Δ)
+  | nil => nil
+  | cons x h => cons ⟨ρ x.name, x.ty⟩ (rename hΓ.tail h)
+  | skip hxn h => skip
+    (hxn.rename (hΓ.wk (skip hxn h)) (hΓ.wk (cons _ h)).head_ne)
+    (rename hΓ.tail h)
+
+def InstSet.Tm.rename {Φ : InstSet (Ty α)} {Γ : Ctx ν (Ty α)} {a : Ty α}
+  {ρ : ν → ν'} (hρ : Γ.InjOn ρ) : Φ.Tm p Γ a → Φ.Tm p (Γ.rename ρ) a
+  | var p h' => @var _ _ _ _ ⟨ρ _, _⟩ p (h'.rename hρ)
+  | op f e => op f (e.rename hρ)
+  | pair p l r => pair p (l.rename hρ) (r.rename hρ)
+  | unit p => unit p
+
+inductive InstSet.Body.InjOn {Φ : InstSet (Ty α)} (ρ : ν → ν')
+  : {Γ Δ: Ctx ν (Ty α)} → Φ.Body p Γ Δ → Prop
+  | nil {Γ Δ: Ctx ν (Ty α)} (h: Γ.Wk Δ): Γ.InjOn ρ → Body.InjOn ρ (Body.nil p h)
+  | let1 {b: Φ.Body p (⟨x, A⟩::Γ) Δ} (e: Φ.Tm p Γ A): b.InjOn ρ → (b.let1 e).InjOn ρ
+  | let2 {b: Φ.Body p (⟨x, A⟩::⟨y, B⟩::Γ) Δ} (e: Φ.Tm p Γ (Ty.pair A B)):
+    b.InjOn ρ → (b.let2 e).InjOn ρ
+
+def InstSet.Body.InjOn.entry {Φ : InstSet (Ty α)} {Γ Δ : Ctx ν (Ty α)} {p}
+  {b : Φ.Body p Γ Δ} {ρ : ν → ν'} : b.InjOn ρ → Γ.InjOn ρ
+  | nil _ h => h
+  | let1 _ h => h.entry.tail
+  | let2 _ h => h.entry.tail.tail
+
+def InstSet.Body.InjOn.exit {Φ : InstSet (Ty α)} {Γ Δ : Ctx ν (Ty α)} {p}
+  {b : Φ.Body p Γ Δ} {ρ : ν → ν'} : b.InjOn ρ → Δ.InjOn ρ
+  | nil w h => h.wk w
+  | let1 _ h => h.exit
+  | let2 _ h => h.exit
+
+--TODO: InstSet.InjOn case helpers?
+def InstSet.Body.rename {Φ : InstSet (Ty α)} {Γ Δ : Ctx ν (Ty α)}
+  {ρ : ν → ν'} : {b : Φ.Body p Γ Δ} → b.InjOn ρ → Φ.Body p (Γ.rename ρ) (Δ.rename ρ)
+  | nil _ h, hρ => nil _ (h.rename (by cases hρ; assumption))
+  | let1 e b, hρ => let1 (e.rename hρ.entry) (b.rename (by cases hρ; assumption))
+  | let2 e b, hρ => let2 (e.rename hρ.entry) (b.rename (by cases hρ; assumption))
+
+def Ctx.EqOn (ρ₁ ρ₂ : ν → ν') (Γ : Ctx ν α): Prop
+  := Set.EqOn ρ₁ ρ₂ { x : ν | x ∈ Γ.names }
+
+theorem Ctx.EqOn.head {ρ₁ ρ₂ : ν → ν'} {v} {Γ : Ctx ν α} (h : Ctx.EqOn ρ₁ ρ₂ (v::Γ))
+  : ρ₁ v.name = ρ₂ v.name
+  := h (by simp)
+
+theorem Ctx.EqOn.tail {ρ₁ ρ₂ : ν → ν'} {v} {Γ : Ctx ν α} (h : Ctx.EqOn ρ₁ ρ₂ (v::Γ))
+  : Ctx.EqOn ρ₁ ρ₂ Γ
+  := λ _ hx => h (hx.tail _)
+
+theorem Ctx.rename_id: (Γ : Ctx ν α) → Γ.rename id = Γ
+  | [] => rfl
+  | _::Γ => congrArg _ (rename_id Γ)
+
+theorem Ctx.EqOn.rename {ρ₁ ρ₂ : ν → ν'} {Γ : Ctx ν α} (hΓ : Γ.EqOn ρ₁ ρ₂)
+  : Γ.rename ρ₁ = Γ.rename ρ₂
+  := List.map_congr (λ_ hx => Var.rename_eq _ _ _  (hΓ (List.mem_map_of_mem _ hx)))
+
+theorem Ctx.EqOn.rename_id {ρ : ν → ν} {Γ : Ctx ν α} (hΓ : Γ.EqOn ρ id)
+  : Γ.rename ρ = Γ
+  := hΓ.rename.trans Γ.rename_id
+
+structure InstSet.Body.RnOn {Φ : InstSet (Ty α)} (ρ : ν → ν) {Γ Δ : Ctx ν (Ty α)}
+  (b: Φ.Body p Γ Δ) : Prop where
+  injOn: b.InjOn ρ
+  entry: Γ.EqOn ρ id
+  exit: Δ.EqOn ρ id
+
+def InstSet.Body.alpha {Φ : InstSet (Ty α)} {Γ Δ : Ctx ν (Ty α)}
+  {ρ : ν → ν} {b : Φ.Body p Γ Δ} (hb: b.RnOn ρ): Φ.Body p Γ Δ
+  := hb.entry.rename_id ▸ hb.exit.rename_id ▸ b.rename hb.injOn
+
+inductive InstSet.Body.Fresh {Φ : InstSet (Ty α)} (n: ν)
+  : {Γ Δ: Ctx ν (Ty α)} → Φ.Body p Γ Δ → Prop
+  | nil {Γ Δ: Ctx ν (Ty α)} (h: Γ.Wk Δ): Γ.Fresh n → Body.Fresh n (Body.nil p h)
+  | let1 {b: Φ.Body p (⟨x, A⟩::Γ) Δ} (e: Φ.Tm p Γ A): b.Fresh n → (b.let1 e).Fresh n
+  | let2 {b: Φ.Body p (⟨x, A⟩::⟨y, B⟩::Γ) Δ} (e: Φ.Tm p Γ (Ty.pair A B)):
+    b.Fresh n → (b.let2 e).Fresh n
+
+def InstSet.Body.Fresh.entry {Φ : InstSet (Ty α)} {Γ Δ : Ctx ν (Ty α)} {p}
+  {b : Φ.Body p Γ Δ} {n} : b.Fresh n → Γ.Fresh n
+  | nil _ h => h
+  | let1 _ h => h.entry.tail
+  | let2 _ h => h.entry.tail.tail
+
+def InstSet.Body.Fresh.exit {Φ : InstSet (Ty α)} {Γ Δ : Ctx ν (Ty α)} {p}
+  {b : Φ.Body p Γ Δ} {n} : b.Fresh n → Δ.Fresh n
+  | nil w h => h.wk w
+  | let1 _ h => h.exit
+  | let2 _ h => h.exit
+
+def InstSet.Body.defs {Φ : InstSet (Ty α)} {Γ Δ : Ctx ν (Ty α)}
+  : Φ.Body p Γ Δ → List ν
+  | nil _ _ => []
+  | @let1 _ _ _ _ _ _ x _ _ b => x::b.defs
+  | @let2 _ _ _ _ _ _ _ x y _ _ b => x::y::b.defs
+
+inductive InstSet.Body.NotDef {Φ : InstSet (Ty α)} (n: ν)
+  : {Γ Δ : Ctx ν (Ty α)} → Φ.Body p Γ Δ → Prop
+  | nil {Γ Δ: Ctx ν (Ty α)} (h: Γ.Wk Δ): Body.NotDef n (Body.nil p h)
+  | let1 {b: Φ.Body p (⟨x, A⟩::Γ) Δ}: x ≠ n → (e: Φ.Tm p Γ A) →
+    b.NotDef n → (b.let1 e).NotDef n
+  | let2 {b: Φ.Body p (⟨x, A⟩::⟨y, B⟩::Γ) Δ}: x ≠ n → y ≠ n →
+    (e: Φ.Tm p Γ (Ty.pair A B)) → b.NotDef n → (b.let2 e).NotDef n
+
+theorem InstSet.Body.NotDef.not_mem_defs {Φ: InstSet (Ty α)} {b: Φ.Body p Γ Δ}
+  : b.NotDef n → n ∉ b.defs
+  | nil _ => by simp [defs]
+  | let1 hx e b => by
+    simp only [defs, List.mem_cons, not_or]
+    exact ⟨hx.symm, b.not_mem_defs⟩
+  | let2 hx hy e b => by
+    simp only [defs, List.mem_cons, not_or]
+    exact ⟨hx.symm, hy.symm, b.not_mem_defs⟩
+
+theorem InstSet.Body.NotDef.of_not_mem_defs {Φ: InstSet (Ty α)} {b: Φ.Body p Γ Δ}
+  : n ∉ b.defs -> b.NotDef n
+  := by induction b with
+  | nil => exact λ_ => NotDef.nil _
+  | let1 _ _ I =>
+    simp only [defs, List.mem_cons, not_or, and_imp]
+    intro hx hn
+    constructor
+    exact Ne.symm hx
+    exact I hn
+  | let2 _ _ I =>
+    simp only [defs, List.mem_cons, not_or, and_imp]
+    intro hx hy hn
+    constructor
+    exact Ne.symm hx
+    exact Ne.symm hy
+    exact I hn
+
+theorem InstSet.Body.NotDef.iff_not_mem_defs {Φ: InstSet (Ty α)} {b: Φ.Body p Γ Δ}
+  : b.NotDef n ↔ n ∉ b.defs
+  := ⟨not_mem_defs, of_not_mem_defs⟩
+
+def InstSet.Body.Fresh.notDef {Φ : InstSet (Ty α)} {Γ Δ : Ctx ν (Ty α)} {p}
+  {b : Φ.Body p Γ Δ} {n} : b.Fresh n → b.NotDef n
+  | nil _ h => NotDef.nil _
+  | let1 _ h => NotDef.let1 h.entry.head _ h.notDef
+  | let2 _ h => NotDef.let2 h.entry.head h.entry.tail.head _ h.notDef
+
+inductive InstSet.Body.SSA {Φ: InstSet (Ty α)}
+  : {Γ Δ: Ctx ν (Ty α)} → Φ.Body p Γ Δ → Prop
+  | nil {Γ Δ: Ctx ν (Ty α)} (h: Γ.Wk Δ): Body.SSA (Body.nil p h)
+  | let1 {b: Φ.Body p (⟨x, A⟩::Γ) Δ}:
+    b.NotDef x → (e: Φ.Tm p Γ A) → b.SSA → (b.let1 e).SSA
+  | let2 {b: Φ.Body p (⟨x, A⟩::⟨y, B⟩::Γ) Δ}:
+    b.NotDef x → b.NotDef y → (e: Φ.Tm p Γ (Ty.pair A B)) → b.SSA → (b.let2 e).SSA
+
+-- theorem InstSet.Body.SSA.rename {Φ: InstSet (Ty α)} {Γ Δ: Ctx ν (Ty α)}
+--   {ρ: ν → ν'} {b: Φ.Body p Γ Δ}
+--   : b.SSA → (hρ : b.InjOn ρ) -> (b.rename hρ).SSA
+--   | nil h, hρ => by simp only [Body.rename]; exact SSA.nil (h.rename hρ.entry) --TODO: defeq?
+--   | let1 hx e b, hρ => by
+--     simp only [Body.rename]
+--     exact SSA.let1 sorry (e.rename hρ.entry) (b.rename (by cases hρ; assumption))
+--   | let2 hx hy e b, hρ => by
+--     simp only [Body.rename]
+--     exact SSA.let2 sorry sorry (e.rename hρ.entry) (b.rename (by cases hρ; assumption))
